Graphplan/Search/Basic.lean
@@ -9,15 +9,18 @@ open STRIPS
 namespace Search
 
 -- A proof that a given sequence of actions is a valid plan for a STRIPS planning problem.
-def is_valid_plan (P : STRIPS_Plan) (actions : List (STRIPS_Operator P.Props)) : Bool :=
+def is_valid_plan {α : Type} (P : STRIPS_Plan α) (actions : List (STRIPS_Operator α)) : Bool :=
   -- let final_state := actions.foldl (fun state op =>
   --   apply_action_if_applicable P op) P.current_state
 
   -- Because I don't really know how to proove that the state has the same type as P.Props,
   -- I will try a different approach.
   let _ := P.prop_decidable -- Proof that Props are decidable
-  let _ : BEq P.Props := instBEqOfDecidableEq -- Proof that Props are comparable
-  let final_state := do
+  let _ : BEq α := instBEqOfDecidableEq -- Proof that Props are comparable
+
+  -- let final_state := do
+
+  let final_state : List α := do
     let mut state := P.current_state
     for op in actions do
       state := apply_action_if_applicable { P with current_state := state } op
@@ -26,54 +29,129 @@ def is_valid_plan (P : STRIPS_Plan) (actions : List (STRIPS_Operator P.Props)) :
   -- Check if any of the goals is fully satisfied in the final state
   P.goal_states.any (fun goal => goal.all (fun p => final_state.contains p))
 
+-- A helper function that generates the last state after applying a list of actions
+def final_state_after_actions {α : Type} (P : STRIPS_Plan α)
+    (actions : List (STRIPS_Operator α)) : List α :=
+  let _ := P.prop_decidable -- Proof that Props are decidable
+  let _ : BEq α := instBEqOfDecidableEq -- Proof that Props are comparable
+  let final_state : List α := do
+    let mut state := P.current_state
+    for op in actions do
+      state := apply_action_if_applicable { P with current_state := state } op
+    state
+  final_state
+  -- with recursion (same result)
+  -- match actions with
+  -- | [] => P.current_state
+  -- | this :: tail =>
+  --   final_state_after_actions { P with current_state := apply_action_if_applicable P this } tail
+
+def is_valid_plan' {α : Type} (P : STRIPS_Plan α)
+    (actions : List (STRIPS_Operator α)) : Prop :=
+  let final_state := final_state_after_actions P actions
+  ∃ goal_state ∈ P.goal_states, goal_state ⊆ final_state
+
+-- Theorem: both definitions of is_valid_plan are equivalent
+theorem is_valid_plan_equiv {α : Type} (P : STRIPS_Plan α)
+    (actions : List (STRIPS_Operator α)) :
+    is_valid_plan P actions = true ↔ is_valid_plan' P actions := by {
+  unfold is_valid_plan is_valid_plan' final_state_after_actions
+  let _ := P.prop_decidable
+  let _ : BEq α := instBEqOfDecidableEq
+  simp_all
+  constructor
+  {
+    intro h_valid
+    obtain ⟨goal_state, h_goal_in_goals, h_goal_subset⟩ := h_valid
+    use goal_state
+    simp_all
+
+    intro goal_state h_goal_in_goals
+    exact List.mem_flatten.mpr (h_goal_subset goal_state h_goal_in_goals)
+  }
+  {
+    intro h_valid
+    obtain ⟨goal_state, h_goal_in_goals, h_goal_subset⟩ := h_valid
+    use goal_state
+    simp_all
+
+    intro x h_x_in_goal
+    exact List.exists_of_mem_flatten (h_goal_subset h_x_in_goal)
+  }
+}
+
+-- Simple helper lemma: if a plan is valid, then another plan, that is identical
+-- but with an one less action at the end that leads to a new state, is also valid if the
+-- new plan has that one new state as its final state.
+theorem valid_plan_extend' {α : Type} (P1 : STRIPS_Plan α)
+    (additional_action : STRIPS_Operator α)
+    (P2 : STRIPS_Plan α := { P1 with
+      current_state := STRIPS.apply_action_if_applicable P1 (additional_action) })
+    (actions1 : List (STRIPS_Operator α))
+    (actions2 : List (STRIPS_Operator α))
+    (h_plan_eq : P2 = { P1 with current_state := STRIPS.apply_action_if_applicable P1 additional_action })
+    (h_actions_eq : actions1 = [additional_action] ++ actions2)
+    (h_valid : is_valid_plan' P2 actions2 = true) :
+    is_valid_plan' P1 actions1 = true := by {
+
+
+      -- simp_all [is_valid_plan, apply_action_if_applicable, apply_action_with_proof]
+      simp_all [is_valid_plan']
+      -- Dig deep into the definitions
+      obtain ⟨goal_state, h_goal_in_goals, h_goal_subset⟩ := h_valid
+      use goal_state
+      simp_all
+
+      unfold final_state_after_actions at *
+      simp_all
+    }
 
 -- A search solution is a sequence of actions that achieves the goal from the initial state.
-structure Solution (P : STRIPS_Plan) where
-  actions : List (STRIPS_Operator P.Props)
+structure Solution {α : Type} (P : STRIPS_Plan α) where
+  actions : List (STRIPS_Operator α)
 
   is_valid : is_valid_plan P actions = true
 
-structure partial_Solution (P : STRIPS_Plan) where
-  actions : List (STRIPS_Operator P.Props)
+structure partial_Solution {α : Type} (P : STRIPS_Plan α) where
+  actions : List (STRIPS_Operator α)
 
 
 -- A helper function that returns all possible actions from the current state.
-def possible_actions {P : STRIPS_Plan} : Array (STRIPS_Operator P.Props) :=
-  P.Actions.filter (fun a => is_applicable a)
+def possible_actions {α : Type} {P : STRIPS_Plan α} : Array (STRIPS_Operator α) :=
+  P.Actions.filter (fun a => is_applicable P a)
 
 
 -- A possible way to represent the search state.
-structure SearchState where
+structure SearchState (α : Type) where
   -- The main plan of the search
-  plan : STRIPS_Plan
+  plan : STRIPS_Plan α
   -- The list of next steps to consider
-  steps_to_consider : List (List plan.Props) -- Note that List is a linked list
+  steps_to_consider : List (List α) -- Note that List is a linked list
   -- to allow for efficient removal of the head action.
 
   -- The fact that a list of props (a step) is decidable for equality
-  step_decidable : DecidableEq (List plan.Props)
+  step_decidable : DecidableEq (List α)
   -- The fact that the List of steps is BEq, that is, it can be compared for equality
-  steps_beq : BEq (List plan.Props)
+  steps_beq : BEq (List α)
   -- The fact that a step is hashable
-  step_hashable : Hashable (List plan.Props)
-
+  step_hashable : Hashable (List α)
   -- The hashmap that maps all known states to their previous state and the action that led to them
-  known_steps : Std.HashMap (List plan.Props) ((List plan.Props) × (STRIPS_Operator plan.Props))
+  known_steps : Std.HashMap (List α) ((List α) × (STRIPS_Operator α))
 
 -- Constructing search states in an easier way
-def mk_search_state (P : STRIPS_Plan) :
-    SearchState :=
+def mk_search_state {α : Type} (P : STRIPS_Plan α) :
+    SearchState α :=
   let plan := P
   let steps_to_consider := [P.current_state]
 
   -- We need to prove BEq and Hashable for the step type (List plan.Props)
   let prop_decidable := P.prop_decidable
-  let step_decidable : DecidableEq (List plan.Props) := by
+  let step_decidable : DecidableEq (List α) := by
     infer_instance
-  let steps_beq : BEq (List plan.Props) := by infer_instance
+  let steps_beq : BEq (List α) := by infer_instance
 
   let prop_hashable := P.prop_hashable
-  let step_hashable : Hashable (List plan.Props) := by
+  let step_hashable : Hashable (List α) := by
     infer_instance
 
   let known_steps := Std.HashMap.emptyWithCapacity 10
@@ -88,7 +166,7 @@ def mk_search_state (P : STRIPS_Plan) :
 -- Whether the goal was reached in the search state
 -- Note that not the entire goal state has to match,
 -- the state only has to contain all the props in one of the goal states.
-def is_goal_reached (s : SearchState) (state : List s.plan.Props) : Bool :=
+def is_goal_reached {α : Type} (s : SearchState α) (state : List α) : Bool :=
   let _ := s.plan.prop_decidable
   ∃ goal_state ∈ s.plan.goal_states, goal_state ⊆ state
 
@@ -101,6 +179,27 @@ def find_in_hashmap? {K V : Type} [BEq K] [Hashable K]
     if k == key then
       return  v
   none
+
+-- Helper function: if is_goal_reached is true, construct a trivial solution:
+-- no actions needed, current state is goal state.
+def trivial_solution_if_goal_reached {α : Type} (s : SearchState α)
+    (h_goal_reached : is_goal_reached s s.plan.current_state = true) :
+    Search.Solution s.plan := by {
+      let _ := s.plan.prop_decidable
+      -- Because the goal is already reached, no actions are needed.
+      let actions : List (STRIPS_Operator α) := []
+      have h_actions : actions = [] := by rfl
+      have h_valid : is_valid_plan s.plan actions = true := by {
+        -- Because the current state already satisfies the goal, the empty action list is valid.
+        simp_all [is_valid_plan, is_goal_reached]
+        obtain ⟨goal_state, h_goal_in_goals, h_goal_subset⟩ := h_goal_reached
+        use goal_state
+        simp_all
+        intro x h_x_in_goal
+        exact h_goal_subset h_x_in_goal
+      }
+      exact { actions := actions, is_valid := h_valid }
+    }
 
 
 end Search
